Deprecate dec_agree
Thanks to Robbert for fixing gen_heap

program_logic/gen_heap.v
@@ -1,28 +1,27 @@
-From iris.algebra Require Import auth gmap frac dec_agree.
+From iris.algebra Require Import auth gmap frac agree.
 From iris.base_logic.lib Require Export own.
 From iris.base_logic.lib Require Import fractional.
 From iris.proofmode Require Import tactics.
 Import uPred.
 
-Definition gen_heapUR (L V : Type) `{Countable L, EqDecision V} : ucmraT :=
-  gmapUR L (prodR fracR (dec_agreeR V)).
-Definition to_gen_heap `{Countable L, EqDecision V} : gmap L V → gen_heapUR L V :=
-  fmap (λ v, (1%Qp, DecAgree v)).
+Definition gen_heapUR (L V : Type) `{Countable L} : ucmraT :=
+  gmapUR L (prodR fracR (agreeR (leibnizC V))).
+Definition to_gen_heap {L V} `{Countable L} : gmap L V → gen_heapUR L V :=
+  fmap (λ v, (1%Qp, to_agree (v : leibnizC V))).
 
 (** The CMRA we need. *)
-Class gen_heapG (L V : Type) (Σ : gFunctors)
-    `{Countable L, EqDecision V} := GenHeapG {
+Class gen_heapG (L V : Type) (Σ : gFunctors) `{Countable L} := GenHeapG {
   gen_heap_inG :> inG Σ (authR (gen_heapUR L V));
   gen_heap_name : gname
 }.
 
-Class gen_heapPreG (L V : Type) (Σ : gFunctors) `{Countable L, EqDecision V} :=
+Class gen_heapPreG (L V : Type) (Σ : gFunctors) `{Countable L} :=
   { gen_heap_preG_inG :> inG Σ (authR (gen_heapUR L V)) }.
 
-Definition gen_heapΣ (L V : Type) `{Countable L, EqDecision V} : gFunctors :=
+Definition gen_heapΣ (L V : Type) `{Countable L} : gFunctors :=
   #[GFunctor (constRF (authR (gen_heapUR L V)))].
 
-Instance subG_gen_heapPreG {Σ} `{Countable L, EqDecision V} :
+Instance subG_gen_heapPreG {Σ L V} `{Countable L} :
   subG (gen_heapΣ L V) Σ → gen_heapPreG L V Σ.
 Proof. intros ?%subG_inG; split; apply _. Qed.
 
@@ -33,7 +32,7 @@ Section definitions.
     own gen_heap_name (● to_gen_heap σ).
 
   Definition mapsto_def (l : L) (q : Qp) (v: V) : iProp Σ :=
-    own gen_heap_name (◯ {[ l := (q, DecAgree v) ]}).
+    own gen_heap_name (◯ {[ l := (q, to_agree (v : leibnizC V)) ]}).
   Definition mapsto_aux : { x | x = @mapsto_def }. by eexists. Qed.
   Definition mapsto := proj1_sig mapsto_aux.
   Definition mapsto_eq : @mapsto = @mapsto_def := proj2_sig mapsto_aux.
@@ -60,14 +59,14 @@ Section gen_heap.
   Lemma lookup_to_gen_heap_None σ l : σ !! l = None → to_gen_heap σ !! l = None.
   Proof. by rewrite /to_gen_heap lookup_fmap=> ->. Qed.
   Lemma gen_heap_singleton_included σ l q v :
-    {[l := (q, DecAgree v)]} ≼ to_gen_heap σ → σ !! l = Some v.
+    {[l := (q, to_agree v)]} ≼ to_gen_heap σ → σ !! l = Some v.
   Proof.
-    rewrite singleton_included=> -[[q' av] [/leibniz_equiv_iff Hl Hqv]].
-    move: Hl. rewrite /to_gen_heap lookup_fmap fmap_Some=> -[v' [Hl [??]]]; subst.
-    by move: Hqv=> /Some_pair_included_total_2 [_ /DecAgree_included ->].
+    rewrite singleton_included=> -[[q' av] []].
+    rewrite /to_gen_heap lookup_fmap fmap_Some_equiv => -[v' [Hl [/= -> ->]]].
+    move=> /Some_pair_included_total_2 [_] /to_agree_included /leibniz_equiv_iff -> //.
   Qed.
   Lemma to_gen_heap_insert l v σ :
-    to_gen_heap (<[l:=v]> σ) = <[l:=(1%Qp, DecAgree v)]> (to_gen_heap σ).
+    to_gen_heap (<[l:=v]> σ) = <[l:=(1%Qp, to_agree (v:leibnizC V))]> (to_gen_heap σ).
   Proof. by rewrite /to_gen_heap fmap_insert. Qed.
 
   (** General properties of mapsto *)
@@ -76,7 +75,7 @@ Section gen_heap.
   Global Instance mapsto_fractional l v : Fractional (λ q, l ↦{q} v)%I.
   Proof.
     intros p q. by rewrite mapsto_eq -own_op -auth_frag_op
-      op_singleton pair_op dec_agree_idemp.
+      op_singleton pair_op agree_idemp.
   Qed.
   Global Instance mapsto_as_fractional l q v :
     AsFractional (l ↦{q} v) (λ q, l ↦{q} v)%I q.
@@ -86,7 +85,7 @@ Section gen_heap.
   Proof.
     rewrite mapsto_eq -own_op -auth_frag_op own_valid discrete_valid.
     f_equiv=> /auth_own_valid /=. rewrite op_singleton singleton_valid pair_op.
-    by move=> [_ /= /dec_agree_op_inv [?]].
+    by intros [_ ?%agree_op_inv%(inj to_agree)%leibniz_equiv].
   Qed.
 
   Global Instance heap_ex_mapsto_fractional l : Fractional (λ q, l ↦{q} -)%I.
@@ -105,8 +104,7 @@ Section gen_heap.
     rewrite mapsto_eq /mapsto_def own_valid !discrete_valid.
     by apply pure_mono=> /auth_own_valid /singleton_valid [??].
   Qed.
-  Lemma mapsto_valid_2 l q1 q2 v1 v2 :
-    l ↦{q1} v1 ∗ l ↦{q2} v2 ⊢ ✓ (q1 + q2)%Qp.
+  Lemma mapsto_valid_2 l q1 q2 v1 v2 : l ↦{q1} v1 ∗ l ↦{q2} v2 ⊢ ✓ (q1 + q2)%Qp.
   Proof.
     iIntros "[H1 H2]". iDestruct (mapsto_agree with "[$H1 $H2]") as %->.
     iApply (mapsto_valid l _ v2). by iFrame.
@@ -118,7 +116,7 @@ Section gen_heap.
     iIntros (?) "Hσ". rewrite /gen_heap_ctx mapsto_eq /mapsto_def.
     iMod (own_update with "Hσ") as "[Hσ Hl]".
     { eapply auth_update_alloc,
-        (alloc_singleton_local_update _ _ (1%Qp, DecAgree v))=> //.
+        (alloc_singleton_local_update _ _ (1%Qp, to_agree (v:leibnizC _)))=> //.
       by apply lookup_to_gen_heap_None. }
     iModIntro. rewrite to_gen_heap_insert. iFrame.
   Qed.
@@ -138,7 +136,7 @@ Section gen_heap.
       as %[Hl%gen_heap_singleton_included _]%auth_valid_discrete_2.
     iMod (own_update_2 with "Hσ Hl") as "[Hσ Hl]".
     { eapply auth_update, singleton_local_update,
-        (exclusive_local_update _ (1%Qp, DecAgree v2))=> //.
+        (exclusive_local_update _ (1%Qp, to_agree (v2:leibnizC _)))=> //.
       by rewrite /to_gen_heap lookup_fmap Hl. }
     iModIntro. rewrite to_gen_heap_insert. iFrame.
   Qed.
